

# Algorithm Improvement Documentation

Fergie

November 14, 2025

## 1 Introduction

This document summarizes the reasoning employed in `new_algorithm.ipynb`, where we argue that  $X_{\text{transformed}} = X_{\text{transformed\_1}}$ . Our scheme is

$$\begin{aligned}\tilde{X} &= H^* D^* X^* = (H_k \otimes H_m) \begin{bmatrix} D_1 & 0 & \cdots & 0 \\ 0 & D_2 & \ddots & \vdots \\ \vdots & \ddots & \ddots & 0 \\ 0 & \cdots & 0 & D_k \end{bmatrix} \begin{bmatrix} X_{1,\text{loc}} \\ X_{2,\text{loc}} \\ \vdots \\ X_{k,\text{loc}} \end{bmatrix} \\ &= (H_k I_k \otimes I_m H_m) \begin{bmatrix} D_1 X_{1,\text{loc}} \\ D_2 X_{2,\text{loc}} \\ \vdots \\ D_k X_{k,\text{loc}} \end{bmatrix} = (H_k \otimes I_m)(I_k \otimes H_m) \begin{bmatrix} D_1 X_{1,\text{loc}} \\ D_2 X_{2,\text{loc}} \\ \vdots \\ D_k X_{k,\text{loc}} \end{bmatrix} \\ &= (H_k \otimes I_m) \begin{bmatrix} H_m & 0 & \cdots & 0 \\ 0 & H_m & \ddots & \vdots \\ \vdots & \ddots & \ddots & 0 \\ 0 & \cdots & 0 & H_m \end{bmatrix}_{k \text{ blocks}} \begin{bmatrix} D_1 X_{1,\text{loc}} \\ D_2 X_{2,\text{loc}} \\ \vdots \\ D_k X_{k,\text{loc}} \end{bmatrix} \\ &= (H_k \otimes I_m) \begin{bmatrix} H_m D_1 X_{1,\text{loc}} \\ H_m D_2 X_{2,\text{loc}} \\ \vdots \\ H_m D_k X_{k,\text{loc}} \end{bmatrix}.\end{aligned}\tag{1}$$

Additionally, inserting a common sampling matrix  $S \in \mathbb{R}^{m \times m}$  before each  $H_m D_k X_{k,\text{loc}}$  yields

$$\begin{aligned}
(H_k \otimes I_m) \begin{bmatrix} S H_m D_1 X_{1,\text{loc}} \\ S H_m D_2 X_{2,\text{loc}} \\ \vdots \\ S H_m D_k X_{k,\text{loc}} \end{bmatrix} &= (H_k \otimes I_m) (I_k \otimes S H_m) \begin{bmatrix} D_1 X_{1,\text{loc}} \\ D_2 X_{2,\text{loc}} \\ \vdots \\ D_k X_{k,\text{loc}} \end{bmatrix} \\
&= (H_k \otimes I_m) (I_k \otimes S) (I_k \otimes H_m) \begin{bmatrix} D_1 X_{1,\text{loc}} \\ \vdots \\ D_k X_{k,\text{loc}} \end{bmatrix} \\
&= (I_k \otimes S) (H_k \otimes I_m) (I_k \otimes H_m) \begin{bmatrix} D_1 X_{1,\text{loc}} \\ \vdots \\ D_k X_{k,\text{loc}} \end{bmatrix} \quad (\text{since } (H_k \otimes I_m)(I_k \otimes S) = (I_k \otimes S)(H_k \otimes I_m)) \\
&= (I_k \otimes S) (H_k \otimes H_m) \begin{bmatrix} D_1 X_{1,\text{loc}} \\ \vdots \\ D_k X_{k,\text{loc}} \end{bmatrix} \\
&=: B H_{km} \begin{bmatrix} D_1 X_{1,\text{loc}} \\ \vdots \\ D_k X_{k,\text{loc}} \end{bmatrix}, \quad \text{where } B := I_k \otimes S, \quad H_{km} := H_k \otimes H_m.
\end{aligned}$$

If each client uses its own sampling matrix  $S_i \in \mathbb{R}^{m \times m}$ ,  $i = 1, \dots, k$ , then

$$\begin{aligned}
(H_k \otimes I_m) \begin{bmatrix} S_1 H_m D_1 X_{1,\text{loc}} \\ S_2 H_m D_2 X_{2,\text{loc}} \\ \vdots \\ S_k H_m D_k X_{k,\text{loc}} \end{bmatrix} &= (H_k \otimes I_m) \begin{bmatrix} S_1 & & \\ & \ddots & \\ & & S_k \end{bmatrix} (I_k \otimes H_m) \begin{bmatrix} D_1 X_{1,\text{loc}} \\ \vdots \\ D_k X_{k,\text{loc}} \end{bmatrix} \\
&= (H_k \otimes I_m) S_{\text{blk}} (I_k \otimes H_m) \begin{bmatrix} D_1 X_{1,\text{loc}} \\ \vdots \\ D_k X_{k,\text{loc}} \end{bmatrix}, \quad \text{where } S_{\text{blk}} := \begin{bmatrix} S_1 & & \\ & \ddots & \\ & & S_k \end{bmatrix}.
\end{aligned}$$

A single global sampling matrix of the form  $B = I_k \otimes S$  would require

$$S_{\text{blk}} = I_k \otimes S = \begin{bmatrix} S & & \\ & \ddots & \\ & & S \end{bmatrix}.$$

$$\text{Thus } S_{\text{blk}} = I_k \otimes S \iff S_1 = S_2 = \dots = S_k = S.$$

If the  $S_i$  are not all identical (i.e.,  $\exists i \neq j : S_i \neq S_j$ ), then

$S_{\text{blk}} \neq I_k \otimes S$  for any  $S$ , so we cannot write

$$(H_k \otimes I_m) S_{\text{blk}} (I_k \otimes H_m) = B H_{km} \begin{bmatrix} D_1 X_{1,\text{loc}} \\ \vdots \\ D_k X_{k,\text{loc}} \end{bmatrix} \quad \text{with a single global } B \text{ of the form } I_k \otimes S.$$